In binary star systems, angular momentum loss is a driving mechanism for the system dynamics. The angular momentum $\vec{J}$ is generally written with the moments of inertia $I$ and the angular velocities $\omega$:

$$\vec{J}=\sum_{i=1}^{2} I_{i} \vec{\omega}_{i}$$

The contributions to the angular momentum from both stars add (orbits in a common direction).

$$\vec{J}=I_{1} \vec{\omega}_{1}+I_{2} \vec{\omega}_{2}$$

$$|J|=m_{1}r_{1}^{2}\omega{1} + m_{2}r_{2}^{2}\omega{2}$$

We know that the stars are orbiting at the same angular velocity, otherwise one would catch up to the other $\omega{1}=\omega{}_{2}=\omega{}$. Also, let us explicitly write that $m_{1} + m_{2}=M$. Let us place the center of mass at the origin so that the 1D equation is 

$$CM=0=\frac{m_{1}r_{1} + m_{2}r_{2<nowiki>}}</nowiki>{M}$$

From this, we find that $m_{1}r_{1} = -m_{2}r_{2}$ or when we substitute the mass ratio $q=\frac{m_{2<nowiki>}}{m_{1}}</nowiki>$, $r_{1} = -qr_{2}$. Note also that, in magnitude $q=\frac{m_{2<nowiki>}}{m_{1}}=\frac{r_{1}}{r_{2}}</nowiki>$. We will call the separation distance from the primary (more massive) star to the secondary (less massive) star $a$.  The distances from the center of mass to each star are denoted $r_{1}$ and $r_{2}$ such that $r_{1}+r_{2}=a$. Along with the previous definition, we can write $a=qr_{2}+r_{2}=r_{2}(q+1)$ or that $r_{2}=\frac{a}{q+1}$. With these definitions in place, we continue reducing $|J|$.

$$|J|=m_{1}(qr_{2})^{2}\omega{1} + m_{2}r_{2}^{2}\omega{2} = m_{2}\bigl( \frac{m_{1<nowiki>}}{m_{2}}</nowiki>q^{2}r_{2}^{2}\omega + r_{2}^{2}\omega \bigr)$$

$$|J|= m_{2} r_{2}^{2}\omega \bigl( \frac{q^{2<nowiki>}}</nowiki>{q} +1\bigr)= m_{2} r_{2}^{2}\omega ( q +1)$$

$$|J|= m_{2} \bigl(\frac{a}{q+1}\bigr)^{2}\omega ( q +1)= m_{2} \bigl(\frac{a^{2<nowiki>}}</nowiki>{q+1}\bigr)\omega$$

$$|J|= m_{2} \bigl(\frac{a^{2<nowiki>}}</nowiki>{(m_{2}/m_{1})+1}\bigr)\omega$$

$$|J|= \frac{m_{2}m_{1}\omega a^{2<nowiki>}}</nowiki>{M}$$

$\omega{}=\frac{2\pi}{P}$, and from Newton's version of Kepler's Third Law that $P=\Bigl( \frac{4\pi^{2}a^{3<nowiki>}}</nowiki>{GM}\Bigr)^{1/2}$. Putting these together, $\omega{}=\bigl( \frac{GM}{a^{3<nowiki>}}</nowiki>\bigr)^{1/2}$.

$$|J|= \frac{m_{2}m_{1} a^{2<nowiki>}}</nowiki>{M}\Bigl(\frac{GM}{a^{3<nowiki>}}</nowiki>\Bigr)^{1/2}$$

$$|J|= m_{1}m_{2} Bigl(\frac{Ga}{M}\Bigr)^{1/2}$$